theories/case_studies/switcher_adequacy.v
@@ -73,7 +73,7 @@ Section helpers_switcher_adequacy.
   Lemma ot_switcher_interp
     (W : WORLD) (C : CmptName) (C_cmpt : cmpt)
     (g_etbl : Locality) (a_etbl: Addr)
-    (args off : nat) (ot : OType) (Nswitcher CNAME : namespace) :
+    (args off : nat) (Nswitcher CNAME : namespace) :
     let b_etbl := (cmpt_exp_tbl_pcc C_cmpt) in
     let b_etbl1 := (cmpt_exp_tbl_cgp C_cmpt) in
     let e_etbl := (cmpt_exp_tbl_entries_end C_cmpt) in
@@ -127,42 +127,5 @@ Section helpers_switcher_adequacy.
     }
     iApply fundamental_execute_entry_point; eauto.
   Qed.
-
-  (* Lemma ot_switcher_interp_entry *)
-  (*   (W : WORLD) (C : CmptName) (C_cmpt : cmpt) *)
-  (*   (a_etbl: Addr) *)
-  (*   (args off : nat) (ot : OType) (Nswitcher CNAME : namespace) : *)
-  (*   let b_etbl := (cmpt_exp_tbl_pcc C_cmpt) in *)
-  (*   let b_etbl1 := (cmpt_exp_tbl_cgp C_cmpt) in *)
-  (*   let e_etbl := (cmpt_exp_tbl_entries_end C_cmpt) in *)
-  (*   let entries_etbl := (cmpt_exp_tbl_entries_start C_cmpt) in *)
-  (*   let b_pcc := (cmpt_b_pcc C_cmpt) in *)
-  (*   let e_pcc := (cmpt_e_pcc C_cmpt) in *)
-  (*   let b_cgp := (cmpt_b_cgp C_cmpt) in *)
-  (*   let e_cgp := (cmpt_e_cgp C_cmpt) in *)
-  (*   (entries_etbl <= a_etbl < e_etbl)%a *)
-  (*   → 0 <= args < 7 *)
-  (*   → na_inv logrel_nais Nswitcher switcher_inv *)
-  (*   ⊢ inv (export_table_PCCN CNAME) (b_etbl ↦ₐ WCap RX Global b_pcc e_pcc b_pcc) *)
-  (*   -∗ inv (export_table_CGPN CNAME) (b_etbl1 ↦ₐ WCap RW Global b_cgp e_cgp b_cgp) *)
-  (*   -∗ inv (export_table_entryN CNAME a_etbl) (a_etbl ↦ₐ WInt (encode_entry_point args off)) *)
-  (*   -∗ seal_pred ot ot_switcher_propC *)
-  (*   -∗ interp W C (WCap RX Global b_pcc e_pcc b_pcc) *)
-  (*   -∗ interp W C (WCap RW Global b_cgp e_cgp b_cgp) *)
-  (*   -∗ WSealed ot_switcher (SCap RO Global b_etbl e_etbl a_etbl) ↦□ₑ args *)
-  (*   -∗ WSealed ot_switcher (SCap RO Local b_etbl e_etbl a_etbl) ↦□ₑ args *)
-  (*   -∗ interp W C (WSealed ot (SCap RO Global b_etbl e_etbl a_etbl)). *)
-  (* Proof. *)
-  (*   intros b_etbl b_etbl1 e_etbl entries_etbl b_pcc e_pcc b_cgp e_cgp Ha_etbl Hargs. *)
-  (*   iIntros "#Hinv_switcher #Hinv_pcc #Hinv_cgp #Hinv_entry *)
-  (*   #Hsealed_pred_ot_switcher #Hinterp_pcc #Hinterp_cgp #Hentry #Hentry'". *)
-
-  (*   iEval (rewrite fixpoint_interp1_eq); iEval (cbn). *)
-  (*   rewrite /interp_sb. *)
-  (*   iFrame "Hsealed_pred_ot_switcher". *)
-  (*   iSplit; first (iPureIntro ; apply persistent_cond_ot_switcher). *)
-  (*   iSplit; first (iIntros (w) ; iApply mono_priv_ot_switcher). *)
-  (*   iSplit; iApply (ot_switcher_interp with "[$] [$] [$] [$] [$] [$]"); eauto. *)
-  (* Qed. *)
 
 End helpers_switcher_adequacy.
